src/Language/PlutusIR/Transform/Rename/DecOpt.v
@@ -1,0 +1,70 @@
+From PlutusCert Require Import
+  Util.List
+  Util.DecOpt
+  Language.PlutusIR
+  (* Language.PlutusIR.DecOpt *)
+  (* Language.PlutusIR.Analysis.Equality.DecOpt *)
+  Language.PlutusIR.Semantics.Static.Theorems.ContextInvariance.AFI
+  Language.PlutusIR.Semantics.Static.Theorems.ContextInvariance.AFI.DecOpt
+  Language.PlutusIR.Transform.Rename.
+
+From QuickChick Require Import QuickChick.
+From CTProxy Require Import CTProxy.
+
+
+
+QCDerive DecOpt for (no_capture x t Γ).
+
+Instance DecOptno_capture_sound x t Γ : DecOptSoundPos (no_capture x t Γ).
+Proof. derive_sound. Qed.
+
+
+
+QCDerive DecOpt for (no_captureA α t Δ).
+
+Instance DecOptno_captureA_sound α t Δ : DecOptSoundPos (no_capture α t Δ).
+Proof. derive_sound. Qed.
+
+
+
+QCDerive DecOpt for (no_ty_capture α τ Δ).
+
+Instance DecOptno_ty_capture_sound α τ Δ : DecOptSoundPos (no_ty_capture α τ Δ).
+Proof. derive_sound. Qed.
+
+
+
+QCDerive DecOpt for (no_ty_capture_constructors α cs Δ).  
+
+Instance DecOptno_ty_capture_constructors_sound α cs Δ : DecOptSoundPos (no_ty_capture_constructors α cs Δ).
+Proof. derive_sound. Qed.
+
+
+
+QCDerive DecOpt for (rename_tvs Δ cs tvs tvs' Δ_tvs).
+
+Instance DecOptrename_tvs_sound Δ cs tvs tvs' Δ_tvs : DecOptSoundPos (rename_tvs Δ cs tvs tvs' Δ_tvs).
+Proof. derive_sound. Qed.
+
+
+
+QCDerive DecOpt for (rename_ty Δ ty ty').
+
+Instance DecOptrename_ty_sound Δ ty ty': DecOptSoundPos (rename_ty Δ ty ty').
+Proof. derive_sound. Qed.
+
+
+
+
+MetaCoq Run (deriveCTProxy rename).
+
+Local Hint Constructors rename rename_binding rename_Bindings_Rec rename_constrs : rename_hints. 
+
+Lemma rename_proxy_sound : rename_proxy_sound_type.
+Proof. deriveCTProxy_sound rename_hints. Qed.
+
+ 
+
+
+QCDerive DecOpt for (rename_proxy Γ Δ tm tm').
+
